Test/civl/inductive-sequentialization/snapshot-scatter-gather-full.bpl
@@ -36,33 +36,39 @@ var {:layer 0,2} r2: [Tid][int]StampedValue;
 var {:linear} {:layer 0,2} pSet: Set Permission;
 
 function {:inline} WholeTidPermission(tid: Tid): Set Permission {
-  Set((lambda {:pool "DirPermission"} x: Permission :: x->t_id == tid && (1 <= x->mem_index) && (x->mem_index <= n)))
+  Set((lambda {:pool "TidPermission"} x: Permission :: x->t_id == tid && (1 <= x->mem_index) && (x->mem_index <= n)))
 }
 
+action {:layer 1} start ({:linear_in} tid: One Tid)
+creates main_f;
+{
+    call create_async(main_f(tid));
+}
 
 // M =  main_f , \elim = read_f, I = Inv_f, M' = main_f'
-action {:layer 1} main_f({:linear_in} tid: One Tid)
+async action {:layer 1} main_f({:linear_in} tid: One Tid)
 refines {:IS_right} main_f' using Inv_f;
 modifies pSet;
 creates read_f;
 {
     var {:linear} sps: Set Permission;
-    assume {:add_to_pool "A", 0} true;
+    // assume {:add_to_pool "A", 0} true;
     call sps := Set_Get(pSet, (lambda x: Permission :: (x->t_id == tid->val) && (1 <= x->mem_index) && (x->mem_index <= n)));
     call create_asyncs((lambda pa:read_f :: (1 <= pa->i) && (pa->i <= n) && pa->perm == One(Permission(tid->val, pa->i))));
 }
 
-async action {:layer 1} gather_f({:linear_in} perm: One Permission)
-modifies pSet;
+async action {:layer 1, 2} gather_f()
+// modifies pSet;
 {
-    call One_Put(pSet, perm);
-    // call Set_Get(pSet(lambda x: Permission :: (x->t_id == tid->val) && (1 <= x->mem_index) && (x->mem_index <= n)));
-    // if (*){
-    assume Set_IsSubset(WholeTidPermission(tid->val), pSet);
-    // }
+    // call One_Put(pSet, perm);
+    // // call Set_Get(pSet(lambda x: Permission :: (x->t_id == tid->val) && (1 <= x->mem_index) && (x->mem_index <= n)));
+    // // if (*){
+    // assume Set_IsSubset(WholeTidPermission(tid->val), pSet);
+    // // }
 }
 
 action {:layer 2} main_f'({:linear_in} tid: One Tid)
+creates gather_f;
 modifies r1, pSet;
 {
     var {:linear} sps: Set Permission;
@@ -73,13 +79,14 @@ modifies r1, pSet;
     assume (forall i:int :: ((1 <= i && i <= n) ==> (r1[tid->val][i]->ts < mem[i]->ts  || r1[tid->val][i]== mem[i]))); 
     call done_set := Set_Get(sps, (lambda x: Permission :: (x->t_id == tid->val) && (1 <= x->mem_index) && (x->mem_index <= n))); 
     call Set_Put(pSet, done_set);
+    call create_async(gather_f());
+
 }
 
 async action {:layer 1} read_f({:linear_in} perm: One Permission, i: int)
 creates read_f, gather_f;
 modifies r1, pSet;
 {
-    // var {:linear} sps2: Set Permission;
     var {:pool "K"} k:int;
     var {:pool "V"} v:Value;
 
@@ -90,18 +97,39 @@ modifies r1, pSet;
     } else {
         r1[perm->val->t_id][i]:= mem[i];
     }
-    // call Set_Put(pSet, Set((lambda x: Permission :: (x->t_id == perm->val->t_id) && (i == x->mem_index) )));
     call One_Put(pSet, perm);
 
-    //case X 
-    if (Set_IsSubset(WholeTidPermission(perm->val->t_id), pSet)){
-        then: create async main_s
+    if (beta = Set_IsSubset(WholeTidPermission(perm->val->t_id), pSet)){
+        // call create_async(main_s(perm->val->t_id));
+        call create_async(gather_f());
     }
-    else{
-        
+}
+// check 1: assume beta, any pa is in \elim or creates no pas
+// check 2: assume not beta, any pa is not in \elim or create no pas
+// beta = true as default (whole action is a right mover)
+
+// chi = not beta (maybe)
+
+// inconsistency: normal action execution , not beta action execution should be inconsistent together.
+
+
+//specify negation : specify the exit (chi)
+
+async action {:layer 1} alpha_read_f({:linear_in} perm: One Permission, i: int)
+creates read_f;
+modifies r1, pSet;
+{
+    var {:pool "K"} k:int;
+    var {:pool "V"} v:Value;
+
+    if (*) {
+        assume {:add_to_pool "K", mem[i]->ts, k} {:add_to_pool "V", mem[i]->value, v} true;
+        assume k < mem[i]->ts; 
+        r1[perm->val->t_id][i]:= StampedValue(k, v);
+    } else {
+        r1[perm->val->t_id][i]:= mem[i];
     }
-    // call sps2 = Set_Get(pSet)
-    // call create_async(gather_f(perm));
+    call One_Put(pSet, perm);
 }
 
 atomic action {: layer 1,2} write(i: int,v: Value)
@@ -138,61 +166,63 @@ creates read_f, gather_f;
 
 // // ISL part
 
+
+
 // M =  main_s , \elim = read_s, I = Inv_s, M' = main_s'
-action {:layer 1} main_s({:linear_in} tid: One Tid)
-refines {:IS_left} main_s' using Inv_s;
-modifies pSet;
-creates read_s;
-{
-    var {:linear} sps: Set Permission;
+// async action {:layer 1} main_s({:linear_in} tid: One Tid)
+// refines {:IS_left} main_s' using Inv_s;
+// modifies pSet;
+// creates read_s;
+// {
+//     var {:linear} sps: Set Permission;
 
-    assume {:add_to_pool "A", 0} true;
-    call sps := Set_Get(pSet, (lambda x: Permission :: (x->t_id == tid->val) && (1 <= x->mem_index) && (x->mem_index <= n)));
-    call create_asyncs((lambda pa:read_s :: (1 <= pa->i) && (pa->i <= n) && pa->perm == One(Permission(tid->val, pa->i))));
-}
+//     assume {:add_to_pool "A", 0} true;
+//     call sps := Set_Get(pSet, (lambda x: Permission :: (x->t_id == tid->val) && (1 <= x->mem_index) && (x->mem_index <= n)));
+//     call create_asyncs((lambda pa:read_s :: (1 <= pa->i) && (pa->i <= n) && pa->perm == One(Permission(tid->val, pa->i))));
+// }
 
-action {:layer 2} main_s'({:linear_in} tid: One Tid)
-modifies r2, pSet;
-{
-    var {:linear} sps: Set Permission;
+// action {:layer 2} main_s'({:linear_in} tid: One Tid)
+// modifies r2, pSet;
+// {
+//     var {:linear} sps: Set Permission;
 
-    call sps := Set_Get(pSet, (lambda x: Permission :: (x->t_id == tid->val) && (1 <= x->mem_index) && (x->mem_index <= n)));
-    havoc r2;
-    assume (forall i:int :: ((1 <= i && i <= n) ==> (r2[tid->val][i]->ts > mem[i]->ts  || r2[tid->val][i] == mem[i]))); 
-}
+//     call sps := Set_Get(pSet, (lambda x: Permission :: (x->t_id == tid->val) && (1 <= x->mem_index) && (x->mem_index <= n)));
+//     havoc r2;
+//     assume (forall i:int :: ((1 <= i && i <= n) ==> (r2[tid->val][i]->ts > mem[i]->ts  || r2[tid->val][i] == mem[i]))); 
+// }
 
-async action {:layer 1} read_s({:linear_in} perm: One Permission, i: int)
-creates read_s;
-modifies r2;
-{
-    var {:pool "K"} k:int;
-    var {:pool "V"} v:Value;
+// async action {:layer 1} read_s({:linear_in} perm: One Permission, i: int)
+// creates read_s;
+// modifies r2;
+// {
+//     var {:pool "K"} k:int;
+//     var {:pool "V"} v:Value;
 
-    if (*) {
-        assume {:add_to_pool "K", mem[i]->ts, k} {:add_to_pool "V", mem[i]->value, v} true;
-        assume k > mem[i]->ts; 
-        r2[perm->val->t_id][i] := StampedValue(k, v);
-    } else {
-        r2[perm->val->t_id][i] := mem[i];
-    }
-}
+//     if (*) {
+//         assume {:add_to_pool "K", mem[i]->ts, k} {:add_to_pool "V", mem[i]->value, v} true;
+//         assume k > mem[i]->ts; 
+//         r2[perm->val->t_id][i] := StampedValue(k, v);
+//     } else {
+//         r2[perm->val->t_id][i] := mem[i];
+//     }
+// }
 
-action {:layer 1} Inv_s({:linear_in} tid: One Tid)
-modifies r2, pSet;
-creates read_s;
-{
-    var {:pool "A"} j: int;
-    var {:linear} sps: Set Permission;
-    var choice: read_s;
+// action {:layer 1} Inv_s({:linear_in} tid: One Tid)
+// modifies r2, pSet;
+// creates read_s;
+// {
+//     var {:pool "A"} j: int;
+//     var {:linear} sps: Set Permission;
+//     var choice: read_s;
 
-    call sps := Set_Get(pSet, (lambda x: Permission :: (x->t_id == tid->val) && (1 <= x->mem_index) && (x->mem_index <= n)));
-    assume {:add_to_pool "A", j+1} 0 <= j && j <= n;
-    havoc r2;
-    assume (forall i:int :: ((1 <= i && i <= j) ==> (r2[tid->val][i]->ts > mem[i]->ts || r2[tid->val][i] == mem[i]))); 
-    if (j < n){
-        choice := read_s(One(Permission(tid->val, j+1)), j+1);
-        assume {:add_to_pool "C", choice} true;
-        call create_asyncs((lambda {:pool "C" } pa:read_s :: ((j+1) <= pa->i) && (pa->i <= n) && pa->perm == One(Permission(tid->val, pa->i))));
-        call set_choice(choice);
-    }
-}
+//     call sps := Set_Get(pSet, (lambda x: Permission :: (x->t_id == tid->val) && (1 <= x->mem_index) && (x->mem_index <= n)));
+//     assume {:add_to_pool "A", j+1} 0 <= j && j <= n;
+//     havoc r2;
+//     assume (forall i:int :: ((1 <= i && i <= j) ==> (r2[tid->val][i]->ts > mem[i]->ts || r2[tid->val][i] == mem[i]))); 
+//     if (j < n){
+//         choice := read_s(One(Permission(tid->val, j+1)), j+1);
+//         assume {:add_to_pool "C", choice} true;
+//         call create_asyncs((lambda {:pool "C" } pa:read_s :: ((j+1) <= pa->i) && (pa->i <= n) && pa->perm == One(Permission(tid->val, pa->i))));
+//         call set_choice(choice);
+//     }
+// }
