Test/civl/inductive-sequentialization/snapshot-scatter-gather-full-old.bpl
@@ -1,0 +1,219 @@
+// RUN: %parallel-boogie "%s" > "%t"
+// RUN: %diff "%s.expect" "%t"
+
+type Value;
+
+type Tid;
+
+datatype StampedValue {
+  StampedValue(ts: int, value: Value)
+} 
+
+datatype Permission {
+    Permission(t_id: Tid, mem_index: int)
+}
+
+// permissions need to put back in globals to retry later
+// how to know scan ended
+// if r1 == r2, return snapshot 
+
+
+// implement one iteration
+// first scan, second scan 
+// if it succeeds then good, otherwise nothing.
+
+
+
+// prove that snapshot is correct if it succeeds.
+// make it retryable anyway
+
+const n: int;
+axiom n >= 1;
+
+var {:layer 0,2} mem: [int]StampedValue;
+var {:layer 0,2} r1: [Tid][int]StampedValue;  
+var {:layer 0,2} r2: [Tid][int]StampedValue; 
+var {:linear} {:layer 0,2} pSet: Set Permission;
+
+function {:inline} WholeTidPermission(tid: Tid): Set Permission {
+  Set((lambda {:pool "DirPermission"} x: Permission :: x->t_id == tid && (1 <= x->mem_index) && (x->mem_index <= n)))
+}
+
+action start({:linear_in} tid: One Tid)
+{
+    call sps := Set_Get(pSet, (lambda x: Permission :: (x->t_id == tid->val) && (1 <= x->mem_index) && (x->mem_index <= n)));
+    async main_f(tid, sps); 
+}
+
+
+// M =  main_f , \elim = read_f, I = Inv_f, M' = main_f'
+action {:layer 1} main_f({:linear_in} tid: One Tid, sps)
+refines {:IS_right} main_f' using Inv_f;
+modifies pSet;
+creates read_f;
+{
+    // var {:linear} sps: Set Permission;
+    assume {:add_to_pool "A", 0} true;
+    // call sps := Set_Get(pSet, (lambda x: Permission :: (x->t_id == tid->val) && (1 <= x->mem_index) && (x->mem_index <= n)));
+    call create_asyncs((lambda pa:read_f :: (1 <= pa->i) && (pa->i <= n) && pa->perm == One(Permission(tid->val, pa->i))));
+}
+
+async action {:layer 1} gather_f({:linear_in} perm: One Permission)
+modifies pSet;
+{
+    call One_Put(pSet, perm);
+    // call Set_Get(pSet(lambda x: Permission :: (x->t_id == tid->val) && (1 <= x->mem_index) && (x->mem_index <= n)));
+    // if (*){
+    assume Set_IsSubset(WholeTidPermission(tid->val), pSet);
+    // }
+}
+
+action {:layer 2} main_f'({:linear_in} tid: One Tid, )
+modifies r1, pSet;
+{
+    var {:linear} sps: Set Permission;
+    var {:linear} done_set: Set Permission;
+
+    call sps := Set_Get(pSet, (lambda x: Permission :: (x->t_id == tid->val) && (1 <= x->mem_index) && (x->mem_index <= n)));
+    havoc r1;
+    assume (forall i:int :: ((1 <= i && i <= n) ==> (r1[tid->val][i]->ts < mem[i]->ts  || r1[tid->val][i]== mem[i]))); 
+    call done_set := Set_Get(sps, (lambda x: Permission :: (x->t_id == tid->val) && (1 <= x->mem_index) && (x->mem_index <= n))); 
+    call Set_Put(pSet, done_set);
+}
+
+// implementation:
+// 1. alpha
+// 2. check right mover check only for alpha. (For now let the user provide alpha as a helper action)
+// Start with this: 3. check that permission are only put in globals, not taken (for all actions) - can we do it only for eliminated actions?
+// 4. inconsistency check (total D). Construct X (chi). 
+
+// set of initial states from which an action executes successfully without blocking (chi is this without the transitions from alpha(A))
+
+// alright this is a good place. Now let's get to work. 
+// to construct chi, we take all g.l such that A succeeds (does not fail or block) - J, and then we take all g.l such that alpha(A) succeeds - I
+
+// is J - I equal to X ? 
+
+
+async action {:layer 1} {:alpha "read_f_alpha"} read_f({:linear_in} perm: One Permission, i: int)
+creates read_f, gather_f;
+modifies r1, pSet;
+{
+    // gate = 
+    // var {:linear} sps2: Set Permission;
+    var {:pool "K"} k:int;
+    var {:pool "V"} v:Value;
+
+    if (*) {
+        assume {:add_to_pool "K", mem[i]->ts, k} {:add_to_pool "V", mem[i]->value, v} true;
+        assume k < mem[i]->ts; 
+        r1[perm->val->t_id][i]:= StampedValue(k, v);
+    } else {
+        r1[perm->val->t_id][i]:= mem[i];
+    }
+    // call Set_Put(pSet, Set((lambda x: Permission :: (x->t_id == perm->val->t_id) && (i == x->mem_index) )));
+    call One_Put(pSet, perm);
+
+    //case X 
+    if (Set_IsSubset(WholeTidPermission(perm->val->t_id), pSet)){
+        then: create async main_s
+    }
+    else{
+        
+    }
+    // call sps2 = Set_Get(pSet)
+    // call create_async(gather_f(perm));
+}
+
+atomic action {: layer 1,2} write(i: int,v: Value)
+modifies mem;
+{
+    var x: StampedValue;
+
+    x := mem[i];
+    mem[i] := StampedValue(x->ts + 1, v);
+}
+
+action {:layer 1} Inv_f({:linear_in} tid: One Tid)
+modifies r1, pSet;
+creates read_f, gather_f;
+{
+    var {:pool "A"} j: int;
+    var {:linear} sps: Set Permission;
+    var {:linear} done_set: Set Permission;
+    var choice: read_f;
+
+    call sps := Set_Get(pSet, (lambda x: Permission :: (x->t_id == tid->val) && (1 <= x->mem_index) && (x->mem_index <= n)));
+    assume {:add_to_pool "A", j+1, 0} 0 <= j && j <= n;
+    havoc r1;
+    assume (forall i:int :: ((1 <= i && i <= j) ==> (r1[tid->val][i]->ts < mem[i]->ts || r1[tid->val][i]== mem[i]))); 
+    call done_set := Set_Get(sps, (lambda x: Permission :: (x->t_id == tid->val) && (1 <= x->mem_index) && (x->mem_index <= j))); 
+    call Set_Put(pSet, done_set);
+    if (j < n){
+        choice := read_f(One(Permission(tid->val, j+1)), j+1);
+        assume {:add_to_pool "C", choice} true;
+        call create_asyncs((lambda {:pool "C" } pa:read_f :: ((j+1) <= pa->i) && (pa->i <= n) && pa->perm == One(Permission(tid->val, pa->i))));
+        call set_choice(choice);
+    }
+}
+
+// // ISL part
+
+// M =  main_s , \elim = read_s, I = Inv_s, M' = main_s'
+action {:layer 1} main_s({:linear_in} tid: One Tid)
+refines {:IS_left} main_s' using Inv_s;
+modifies pSet;
+creates read_s;
+{
+    var {:linear} sps: Set Permission;
+
+    assume {:add_to_pool "A", 0} true;
+    call sps := Set_Get(pSet, (lambda x: Permission :: (x->t_id == tid->val) && (1 <= x->mem_index) && (x->mem_index <= n)));
+    call create_asyncs((lambda pa:read_s :: (1 <= pa->i) && (pa->i <= n) && pa->perm == One(Permission(tid->val, pa->i))));
+}
+
+action {:layer 2} main_s'({:linear_in} tid: One Tid)
+modifies r2, pSet;
+{
+    var {:linear} sps: Set Permission;
+
+    call sps := Set_Get(pSet, (lambda x: Permission :: (x->t_id == tid->val) && (1 <= x->mem_index) && (x->mem_index <= n)));
+    havoc r2;
+    assume (forall i:int :: ((1 <= i && i <= n) ==> (r2[tid->val][i]->ts > mem[i]->ts  || r2[tid->val][i] == mem[i]))); 
+}
+
+async action {:layer 1} read_s({:linear_in} perm: One Permission, i: int)
+creates read_s;
+modifies r2;
+{
+    var {:pool "K"} k:int;
+    var {:pool "V"} v:Value;
+
+    if (*) {
+        assume {:add_to_pool "K", mem[i]->ts, k} {:add_to_pool "V", mem[i]->value, v} true;
+        assume k > mem[i]->ts; 
+        r2[perm->val->t_id][i] := StampedValue(k, v);
+    } else {
+        r2[perm->val->t_id][i] := mem[i];
+    }
+}
+
+action {:layer 1} Inv_s({:linear_in} tid: One Tid)
+modifies r2, pSet;
+creates read_s;
+{
+    var {:pool "A"} j: int;
+    var {:linear} sps: Set Permission;
+    var choice: read_s;
+
+    call sps := Set_Get(pSet, (lambda x: Permission :: (x->t_id == tid->val) && (1 <= x->mem_index) && (x->mem_index <= n)));
+    assume {:add_to_pool "A", j+1} 0 <= j && j <= n;
+    havoc r2;
+    assume (forall i:int :: ((1 <= i && i <= j) ==> (r2[tid->val][i]->ts > mem[i]->ts || r2[tid->val][i] == mem[i]))); 
+    if (j < n){
+        choice := read_s(One(Permission(tid->val, j+1)), j+1);
+        assume {:add_to_pool "C", choice} true;
+        call create_asyncs((lambda {:pool "C" } pa:read_s :: ((j+1) <= pa->i) && (pa->i <= n) && pa->perm == One(Permission(tid->val, pa->i))));
+        call set_choice(choice);
+    }
+}
